temporary fixes on hoare proofs + added in the actual proofs from the demo repo

while-lang/LoVe/whilelang.lean
@@ -67,6 +67,8 @@ theorem silly_from_1_BigStep :
       apply BigStep.while_false
       simp
 
+/- TODO: Find way to rewrite goal using inductive def -/
+
 theorem BigStep_deterministic {Ss l r} (hl: Ss ⟹ l)
   (hr: Ss ⟹ r):
     l = r := by
@@ -94,43 +96,5 @@ theorem BigStep_deterministic {Ss l r} (hl: Ss ⟹ l)
             | refl => cases iHRestS hRestT with
               | refl => rfl
           | while_false => aesop
-
-def PartialHoare (P : State → Prop) (S : Stmt)
-  (Q : State → Prop) : Prop :=
-    ∀s t, P s → (S, s) ⇒ t → Q t
--- Type issue with (S,s), may need 2 define as variable
--- ask prof fremont?
-
-theorem skip_intro {P} :
-  {* P *}(Stmt.skip){* P *}
--- Lean issue? may need to define/dig thru lovelib
-
-
-theorem assign_intro (P) {x a} :
-  {* P (s[x ↦ a s])*}(Stmt.assign x a){* P *}
-
-theorem seq_intro {P Q R S T}
-  (hS: {*P*}(S){*R*})
-  (hT: {*R*}(T){*Q*}) :
-  {* P *} (S; T) {* Q *}
-
-theorem if_intro {P B S Q T}
-  (h: {fun s ↦ P s ∧ B s} (S) {Q})
-  (hb:{fun s ↦ P s ∧ ¬B s} (S) {Q}) :
-  {* P *} (Stmt.ifThenElse B S T) {* Q *}
-
-theorem while_intro (P) {B S}
-  (hS: {* fun s ↦ P s ∧ B s *} (S) {* P *}) :
-    {* P *} (Stmt.whileDo B S) {* fun s ↦ P s ∧ ¬ B s *}
-
-theorem consequence {P P' Q Q' S}
-  (hP: P' s → P s)
-  (hQ: Q → Q')
-  (hS: {*P*} (S) {*Q*}) :
-  {* P' *} (S) {* Q' *}
-
--- maybe try lovelib with deeper arithmetic embeddings?
--- see if it helps
--- maybe ask on zulip or consult documentation
 
 end LoVe
