while-lang/LoVe/hoare.lean
@@ -1,0 +1,120 @@
+import LoVe.LoVelib
+import LoVe.Demo9
+
+set_option autoImplicit false
+set_option tactic.hygienic false
+
+open Lean
+open Lean.Meta
+open Lean.Elab.Tactic
+
+namespace LoVe
+
+
+-- inductive Stmt : Type where
+--   | skip       : Stmt
+--   | assign     : String → (State → ℕ) → Stmt
+--   | seq        : Stmt → Stmt → Stmt
+--   | ifThenElse : (State → Prop) → Stmt → Stmt → Stmt
+--   | whileDo    : (State → Prop) → Stmt → Stmt
+-- infixr:90 "; " => Stmt.seq
+
+
+
+
+def PartialHoare (P : State → Prop) (S : Stmt)
+  (Q : State → Prop) : Prop :=
+    ∀s t, P s → (S, s) ⟹ t → Q t
+-- Type issue with (S,s), may need 2 define as variable
+-- ask prof fremont?
+-- for some reason importing the demo file fixes this
+
+macro "{*" P:term " *} " "(" S:term ")" " {* " Q:term " *}" : term =>
+  `(PartialHoare $P $S $Q)
+
+namespace PartialHoare
+
+theorem skip_intro {P} :
+  {* P *}(Stmt.skip){* P *} :=
+  by
+    intro s t hs hst
+    cases hst
+    assumption
+
+
+
+theorem assign_intro (P) {x a} :
+  {*fun s ↦ P (s[x ↦ a s])*}(Stmt.assign x a){* P *} :=
+  by
+    intro s t P' hst
+    cases hst with
+    | assign => assumption
+
+theorem seq_intro {P Q R S T}
+  (hS: {*P*}(S){*R*})
+  (hT: {*R*}(T){*Q*}) :
+  {* P *} (S; T) {* Q *} :=
+  by
+    intro s t hs hst
+    cases hst with
+    | seq _ _ _ u d hS' hT' =>
+      apply hT
+      { apply hS
+        { exact hs }
+        { assumption } }
+      { assumption }
+
+theorem if_intro {P B S Q T}
+  (h: {* fun s ↦ P s ∧ B s *} (S) {* Q*})
+  (hb:{* fun s ↦ P s ∧ ¬B s *} (S) {* Q *}) :
+  {* P *} (Stmt.ifThenElse B S T) {* Q *} :=
+  by
+    intro s t hs hst
+    cases hst with
+    | if_true _ _ _ _ _ hB hS' =>
+      apply hS
+      exact And.intro hs hB
+      assumption
+    | if_false _ _ _ _ _ hB hT' =>
+      apply hT
+      exact And.intro hs hB
+      assumption
+
+theorem while_intro (P) {B S}
+    (h : {* fun s ↦ P s ∧ B s *} (S) {* P *}) :
+  {* P *} (Stmt.whileDo B S) {* fun s ↦ P s ∧ ¬ B s *} :=
+  by
+    intro s t hs hst
+    generalize ws_eq : (Stmt.whileDo B S, s) = Ss
+    rw [ws_eq] at hst
+    induction hst generalizing s with
+    | skip s'                       => cases ws_eq
+    | assign x a s'                 => cases ws_eq
+    | seq S T s' t' u hS hT ih      => cases ws_eq
+    | if_true B S T s' t' hB hS ih  => cases ws_eq
+    | if_false B S T s' t' hB hT ih => cases ws_eq
+    | while_true B' S' s' t' u hB' hS hw ih_hS ih_hw =>
+      cases ws_eq
+      apply ih_hw
+      { apply h
+        { apply And.intro <;>
+            assumption }
+        { exact hS } }
+      { rfl }
+    | while_false B' S' s' hB'      =>
+      cases ws_eq
+      aesop
+
+theorem consequence {P P' Q Q' S}
+    (h : {* P *} (S) {* Q *}) (hp : ∀s, P' s → P s)
+    (hq : ∀s, Q s → Q' s) :
+  {* P' *} (S) {* Q' *} :=
+  fix s t : State
+  assume hs : P' s
+  assume hst : (S, s) ⟹ t
+  show Q' t from
+    hq _ (h s t (hp s hs) hst)
+
+
+end PartialHoare
+end LoVe
